move things around and get rid of "live" predicate

systems/ChordCorrectness.v
@@ -21,71 +21,10 @@ Require Import Chord.ChordLabeled.
 Require Import Chord.ChordPromises.
 Require Import Chord.ChordDefinitionLemmas.
 Require Import Chord.ChordLocalProps.
+Require Import Chord.ChordPhaseOne.
 
 Set Bullet Behavior "Strict Subproofs".
 Open Scope nat_scope.
-
-Definition live (gst : global_state) (p : pointer) :=
-  live_node gst (addr_of p) /\
-  wf_ptr p.
-
-Definition live_dec :
-  forall gst p,
-    {live gst p} + {~ live gst p}.
-Proof.
-  unfold live.
-  intros.
-  destruct (live_node_dec gst (addr_of p));
-    destruct (wf_ptr_dec p);
-    tauto.
-Defined.
-
-Lemma live_live_addr :
-  forall gst p,
-    wf_ptr p ->
-    live gst p <-> live_node gst (addr_of p).
-Proof.
-  now unfold live.
-Qed.
-
-Lemma live_intro :
-  forall gst p st,
-    wf_ptr p ->
-    In (addr_of p) (nodes gst) ->
-    ~ In (addr_of p) (failed_nodes gst) ->
-    sigma gst (addr_of p) = Some st ->
-    joined st = true ->
-    live gst p.
-Proof.
-  unfold live.
-  intros.
-  eauto using live_node_characterization.
-Qed.
-
-Lemma live_inv :
-  forall gst p,
-    live gst p ->
-    wf_ptr p /\
-    In (addr_of p) (nodes gst) /\
-    ~ In (addr_of p) (failed_nodes gst) /\
-    exists st, sigma gst (addr_of p) = Some st /\
-          joined st = true.
-Proof.
-  unfold live.
-  intros.
-  inv_prop live_node; auto.
-Qed.
-
-Ltac live_inv :=
-  match goal with
-  | [ H_live : live ?gst ?p |- _ ] =>
-    apply live_inv in H_live;
-      destruct H_live as [?H [?H [?H ?H]]];
-      match goal with
-      | [ H_st : exists st, sigma gst (addr_of p) = Some st |- _ ] =>
-        destruct H_st as [?st]
-      end
-  end.
 
 Definition live_addrs (gst : global_state) : list addr :=
   filter (fun a => Coqlib.proj_sumbool (live_node_dec gst a))
@@ -105,54 +44,6 @@ Definition live_ptrs_with_states (gst : global_state) : list (pointer * data) :=
 Definition full_succs (gst : global_state) (h : pointer) (succs : list pointer) : Prop :=
   length succs = Chord.SUCC_LIST_LEN.
 
-(* cf. zave page 11 *)
-Definition first_succ_is_best_succ (gst : global_state) (h : addr) :=
-  exists st s rest,
-    sigma gst h = Some st /\
-    succ_list st = s :: rest /\
-    best_succ gst h (addr_of s).
-
-Definition all_first_succs_best (gst : global_state) :=
-  forall h,
-    live_node gst h ->
-    first_succ_is_best_succ gst h.
-
-Definition phase_one (o : occurrence) : Prop :=
-  all_first_succs_best (occ_gst o).
-
-(* Defining the error for phase one: the norm approach *)
-Fixpoint succ_list_leading_failed_nodes (failed : list addr) (succs : list pointer) : nat :=
-  match succs with
-  | h :: rest =>
-    if In_dec addr_eq_dec (addr_of h) failed
-    then S (succ_list_leading_failed_nodes failed rest)
-    else 0
-  | [] => 0
-  end.
-
-(* The local error measure for phase one. *)
-Definition leading_failed_succs (h : addr) (gst : global_state) : nat :=
-  match sigma gst h with
-  | Some st =>
-    succ_list_leading_failed_nodes (failed_nodes gst) (succ_list st)
-  | None =>
-    0
-  end.
-
-Definition phase_one_error : global_state -> nat :=
-  global_measure leading_failed_succs.
-
-Lemma maybe_count_failed_nodes_Some :
-  forall gst h st n,
-    leading_failed_succs h gst = n ->
-    sigma gst h = Some st ->
-    succ_list_leading_failed_nodes (failed_nodes gst) (succ_list st) = n.
-Proof.
-  unfold leading_failed_succs.
-  intros.
-  break_match; congruence.
-Qed.
-
 Lemma successor_nodes_valid_state :
   forall gst h p st,
     In p (succ_list st) ->
@@ -164,30 +55,6 @@ Proof.
   intros.
   eapply_prop_hyp successor_nodes_valid @eq; eauto.
   now break_and.
-Qed.
-
-Lemma successor_nodes_valid_inv :
-  forall gst h p st,
-    In p (succ_list st) ->
-    successor_nodes_valid gst ->
-    sigma gst h = Some st ->
-    In (addr_of p) (nodes gst) /\
-    exists pst, sigma gst (addr_of p) = Some pst /\
-           joined pst = true.
-Proof.
-  eauto.
-Qed.
-
-Lemma successor_nodes_valid_live_are_joined :
-  forall gst h st p,
-    live gst p ->
-    successor_nodes_valid gst ->
-    sigma gst h = Some st ->
-    In p (succ_list st) ->
-    live_node gst (addr_of p).
-Proof.
-  intros.
-  now inv_prop live.
 Qed.
 
 Lemma nonempty_succ_lists_always_belong_to_joined_nodes :
@@ -206,7 +73,7 @@ Lemma zero_leading_failed_nodes_leading_node_live :
     sigma gst h = Some st ->
     succ_list st = s :: rest ->
     wf_ptr s ->
-    live gst s.
+    wf_ptr s /\ live_node gst (addr_of s).
 Proof.
   intros.
   repeat find_rewrite.
@@ -220,232 +87,7 @@ Proof.
     apply in_eq.
   }
   find_eapply_lem_hyp successor_nodes_valid_inv; eauto; repeat (break_exists_name pst || break_and).
-  eapply live_intro; eauto.
-Qed.
-
-Lemma zero_leading_failed_nodes_best_succ :
-  forall gst h st s rest,
-    succ_list_leading_failed_nodes (failed_nodes gst) (succ_list st) = 0 ->
-    reachable_st gst ->
-    sigma gst h = Some st ->
-    succ_list st = s :: rest ->
-    wf_ptr s ->
-    live_node gst h ->
-    best_succ gst h (addr_of s).
-Proof.
-  unfold best_succ.
-  intros.
-  exists st.
-  exists [].
-  exists (map addr_of rest).
-  simpl.
-  intuition.
-  - repeat find_rewrite.
-    apply map_cons.
-  - eapply successor_nodes_valid_live_are_joined; eauto.
-    + find_copy_eapply_lem_hyp zero_leading_failed_nodes_leading_node_live; eauto.
-    + apply successor_nodes_always_valid.
-      assumption.
-    + repeat find_rewrite.
-      apply in_eq.
-Qed.
-
-Lemma zero_failed_nodes_total_implies_zero_locally :
-  forall gst h st,
-    phase_one_error gst = 0 ->
-    live_node gst h ->
-    sigma gst h = Some st ->
-    succ_list_leading_failed_nodes (failed_nodes gst) (succ_list st) = 0.
-Proof.
-  unfold phase_one_error in *.
-  intros.
-  cut (leading_failed_succs h gst = 0);
-    eauto using maybe_count_failed_nodes_Some.
-  find_eapply_lem_hyp local_all_zero_global_zero.
-  find_eapply_lem_hyp Forall_forall; eauto.
-  inv_prop live_node; break_and.
-  eauto using in_nodes_not_failed_in_active.
-Qed.
-
-Theorem zero_leading_failed_nodes_implies_all_first_succs_best :
-  forall gst,
-    reachable_st gst ->
-    (* total leading failed nodes says nothing about the length of successor lists *)
-    nonempty_succ_lists gst ->
-    phase_one_error gst = 0 ->
-    all_first_succs_best gst.
-Proof.
-  unfold all_first_succs_best, first_succ_is_best_succ, phase_one_error.
-  intros.
-  find_copy_apply_lem_hyp local_all_zero_global_zero;
-    rewrite Forall_forall in *.
-  inv_prop live_node;
-    repeat (break_and; break_exists_exists).
-  unfold nonempty_succ_lists in *.
-  find_copy_apply_hyp_hyp.
-  destruct (succ_list _) as [| p rest] eqn:?H; [firstorder congruence|].
-  exists p. exists rest.
-  repeat split; auto.
-
-  (* need an (easy) invariant *)
-  assert (wf_ptr p) by eauto using wf_ptr_succ_list_invariant.
-
-  assert (live_node gst h) by eauto.
-  find_copy_apply_lem_hyp zero_failed_nodes_total_implies_zero_locally; auto.
-  eapply zero_leading_failed_nodes_best_succ; eauto.
-Qed.
-
-(*
-if head of succ list is dead
-then we set
-cur_request
-Request dst (message?)
-with cur_request = (make_pointer dst, q, _)
-with q = Stabilize
-with q = Stabilize2
-*)
-
-Definition open_stabilize_request_to (gst : global_state) (h : addr) (dst : addr) : Prop :=
-  open_request_to gst h dst GetPredAndSuccs.
-
-Definition open_stabilize_request (gst : global_state) (h : addr) : Prop :=
-  exists p,
-    open_stabilize_request_to gst h (addr_of p) /\
-    wf_ptr p.
-
-(** If h is a valid node with a first successor s in gst, then h has an open
-    stabilize request to s in gst. *)
-Definition open_stabilize_request_to_first_succ (gst : global_state) (h : addr) : Prop :=
-  forall st dst rest,
-    sigma gst h = Some st ->
-    succ_list st = dst :: rest ->
-    open_stabilize_request_to gst h (addr_of dst).
-
-Lemma open_stabilize_request_to_first_succ_elim :
-  forall gst h st hd rest,
-    open_stabilize_request_to_first_succ gst h ->
-    sigma gst h = Some st ->
-    succ_list st = hd :: rest ->
-    open_stabilize_request_to gst h (addr_of hd).
-Proof.
-  eauto.
-Qed.
-
-Lemma timeout_handler_eff_StartStabilize :
-  forall h st r eff,
-    timeout_handler_eff h st Tick = (r, eff) ->
-    joined st = true /\ cur_request st = None <->
-    eff = StartStabilize.
-Proof.
-  intros.
-  destruct (timeout_handler_eff _ _ _) as [[[[?st' ?ms] ?nts] ?cts] ?eff] eqn:?H.
-  find_apply_lem_hyp timeout_handler_eff_definition; expand_def;
-    repeat find_rewrite; try congruence.
-  find_eapply_lem_hyp tick_handler_definition; expand_def;
-    repeat find_rewrite; firstorder congruence.
-Qed.
-
-Lemma timeout_handler_eff_is_timeout_handler_l :
-  forall h st t res eff,
-    timeout_handler_eff h st t = (res, eff) <->
-    timeout_handler_l h st t = (res, Timeout h t eff).
-Proof.
-  intros.
-  unfold timeout_handler_l.
-  break_let.
-  split; intros; solve_by_inversion.
-Qed.
-
-Lemma loaded_Tick_enabled_when_cur_request_None :
-  forall gst h st,
-    reachable_st gst ->
-    live_node gst h ->
-    sigma gst h = Some st ->
-    cur_request st = None ->
-    In Tick (timeouts gst h) ->
-    enabled (Timeout h Tick StartStabilize) gst.
-Proof.
-  intros.
-  break_live_node.
-  (* replace x from live_node with st *)
-  repeat find_rewrite; find_injection.
-  destruct (timeout_handler_eff h st Tick) as [[[[st' ms] nts] cts] eff] eqn:?H.
-  assert (eff = StartStabilize)
-    by (eapply timeout_handler_eff_StartStabilize; eauto).
-  subst.
-  exists (apply_handler_result h (st', ms, nts, Tick :: cts) [e_timeout h Tick] gst).
-  eapply LTimeout; eauto.
-  - now apply timeout_handler_eff_is_timeout_handler_l.
-  - now constructor.
-Qed.
-
-Definition busy_if_live (h : addr) (occ : occurrence) :=
-  forall st,
-    live_node (occ_gst occ) h ->
-    sigma (occ_gst occ) h = Some st ->
-    cur_request st <> None.
-
-Definition not_busy_if_live (h : addr) (occ : occurrence) :=
-  forall st,
-    live_node (occ_gst occ) h ->
-    sigma (occ_gst occ) h = Some st ->
-    cur_request st = None.
-
-(** the big assumption for inf_often stabilization *)
-Theorem queries_eventually_stop :
-  forall ex h,
-    lb_execution ex ->
-    reachable_st (occ_gst (hd ex)) ->
-    strong_local_fairness ex ->
-    live_node (occ_gst (hd ex)) h ->
-    busy_if_live h (hd ex) ->
-    always (~_ (now circular_wait)) ex ->
-    eventually (now (not_busy_if_live h)) ex.
-Proof.
-  (*         -____-   *)
-Admitted.
-
-Lemma always_busy_or_not_busy :
-  forall h occ,
-    not_busy_if_live h occ \/ busy_if_live h occ.
-Proof.
-  intros.
-  unfold not_busy_if_live, busy_if_live.
-  destruct (sigma (occ_gst occ) h) as [d|];
-   [destruct (cur_request d) eqn:?H|];
-   firstorder congruence.
-Qed.
-
-Lemma not_busy_inf_often :
-  forall h ex,
-    lb_execution ex ->
-    reachable_st (occ_gst (hd ex)) ->
-    strong_local_fairness ex ->
-    live_node (occ_gst (hd ex)) h ->
-    always (~_ (now circular_wait)) ex ->
-    inf_often (now (not_busy_if_live h)) ex.
-Proof.
-  intro.
-  pose proof (always_busy_or_not_busy h) as H_bnb.
-  cofix c.
-  intros.
-  constructor.
-  - pose proof (H_bnb (hd ex)).
-    destruct ex.
-    break_or_hyp.
-    + constructor.
-      assumption.
-    + apply queries_eventually_stop; auto.
-  - destruct ex.
-    simpl.
-    eapply c.
-    + eapply lb_execution_invar; eauto.
-    + destruct ex.
-      eapply reachable_st_lb_execution_cons; eauto.
-    + eapply strong_local_fairness_invar; eauto.
-    + inv_lb_execution.
-      eapply live_node_invariant; eauto.
-    + eapply always_invar; eauto.
+  eauto using live_node_characterization.
 Qed.
 
 Lemma live_node_has_Tick_in_timeouts :
@@ -474,410 +116,7 @@ Proof.
   eapply loaded_Tick_enabled_when_cur_request_None; eauto.
 Qed.
 
-Ltac invar_eauto :=
-  eauto using
-        always_invar,
-        lb_execution_invar,
-        strong_local_fairness_invar,
-        live_node_invariant,
-        labeled_step_is_unlabeled_step,
-        reachableStep,
-        lb_execution_step_one_cons.
-
-Lemma loaded_Tick_inf_enabled :
-  forall h ex,
-    lb_execution ex ->
-    reachable_st (occ_gst (hd ex)) ->
-    strong_local_fairness ex ->
-    live_node (occ_gst (hd ex)) h ->
-    always (~_ (now circular_wait)) ex ->
-    inf_enabled (Timeout h Tick StartStabilize) ex.
-Proof.
-  intros h.
-  pose proof (always_busy_or_not_busy h) as H_bnb.
-  intros.
-  unfold inf_enabled.
-  find_copy_apply_lem_hyp not_busy_inf_often; eauto.
-  lift_inf_often (loaded_Tick_enabled_if_now_not_busy_if_live h);
-    invar_eauto.
-Qed.
-
-Lemma loaded_Tick_inf_often :
-  forall ex h,
-    lb_execution ex ->
-    reachable_st (occ_gst (hd ex)) ->
-    strong_local_fairness ex ->
-    live_node (occ_gst (hd ex)) h ->
-    always (~_ (now circular_wait)) ex ->
-    inf_occurred (Timeout h Tick StartStabilize) ex.
-Proof.
-  auto using loaded_Tick_inf_enabled.
-Qed.
-
-Lemma effective_Tick_sends_request :
-  forall gst gst' h st s1 rest,
-    sigma gst h = Some st ->
-    succ_list st = s1 :: rest ->
-    labeled_step_dynamic gst (Timeout h Tick StartStabilize) gst' ->
-    open_stabilize_request_to gst' h (addr_of s1).
-Proof.
-  intros.
-  inv_labeled_step; clean_up_labeled_step_cases.
-  find_apply_lem_hyp timeout_handler_l_definition; expand_def.
-  find_apply_lem_hyp timeout_handler_eff_definition; expand_def;
-    try congruence.
-  find_injection.
-  find_apply_lem_hyp tick_handler_definition; expand_def;
-    try congruence.
-  unfold add_tick in *; repeat break_let;
-    find_apply_lem_hyp start_query_definition; expand_def.
-  - simpl in *.
-    repeat find_rewrite.
-    find_injection.
-    repeat find_rewrite.
-    simpl in *.
-    find_injection.
-    repeat split; simpl in *;
-      try rewrite update_same in *;
-      repeat eexists;
-      eauto using StabilizeMsg with datatypes.
-  - simpl in *.
-    find_rewrite.
-    find_injection.
-    repeat find_rewrite.
-    discriminate.
-Qed.
-
-Lemma option_map_Some :
-  forall A B (f : A -> B) a b,
-    option_map f a = Some b ->
-    exists a', a = Some a' /\
-          f a' = b.
-Proof.
-  intros.
-  destruct a; simpl in *; try congruence.
-  find_injection.
-  eexists; eauto.
-Qed.
-
-Lemma option_map_None :
-  forall A B (f : A -> B) a,
-    option_map f a = None ->
-    a = None.
-Proof.
-  intros.
-  destruct a; simpl in *; congruence.
-Qed.
-
-Lemma make_request_Stabilize_needs_succ_list :
-  forall h st dst m,
-    make_request h st Stabilize = Some (dst, m) ->
-    exists rest,
-      succ_list st = dst :: rest.
-Proof.
-  intros.
-  unfold make_request in *; simpl in *.
-  find_apply_lem_hyp option_map_Some; break_exists; break_and.
-  find_copy_apply_lem_hyp hd_error_some_nil.
-  destruct (succ_list st) eqn:?H; [discriminate|].
-  simpl in *.
-  tuple_inversion.
-  find_injection.
-  eexists; eauto.
-Qed.
-
-Lemma make_request_Stabilize_None :
-  forall h st,
-    make_request h st Stabilize = None ->
-    succ_list st = [].
-Proof.
-  intros.
-  unfold make_request in *; simpl in *.
-  simpl in *.
-  find_eapply_lem_hyp option_map_None.
-  destruct (succ_list st) eqn:?H; simpl in *; congruence.
-Qed.
-
-Lemma succ_list_preserved_by_Tick :
-  forall gst gst' h st st',
-    labeled_step_dynamic gst (Timeout h Tick StartStabilize) gst' ->
-    sigma gst h = Some st ->
-    sigma gst' h = Some st' ->
-    succ_list st' = succ_list st.
-Proof.
-  intros.
-  inv_labeled_step; clean_up_labeled_step_cases.
-  find_apply_lem_hyp timeout_handler_l_definition; expand_def.
-  find_apply_lem_hyp timeout_handler_eff_definition; expand_def;
-    try congruence.
-  find_injection.
-  find_apply_lem_hyp tick_handler_definition; expand_def;
-    try congruence.
-  rewrite sigma_ahr_updates in *; find_injection.
-  destruct (start_query _ _ _) as [[[?st' ?ms] ?nts] ?cts] eqn:?H.
-  find_eapply_lem_hyp add_tick_definition; expand_def.
-  find_apply_lem_hyp start_query_definition; expand_def;
-    repeat find_rewrite; solve_by_inversion.
-Qed.
-
-Lemma effective_Tick_sends_request' :
-  forall gst gst' h st s1 rest,
-    sigma gst' h = Some st ->
-    succ_list st = s1 :: rest ->
-    labeled_step_dynamic gst (Timeout h Tick StartStabilize) gst' ->
-    open_stabilize_request_to gst' h (addr_of s1).
-Proof.
-  intros.
-  inv_labeled_step; clean_up_labeled_step_cases.
-  find_apply_lem_hyp timeout_handler_l_definition; expand_def.
-  find_apply_lem_hyp timeout_handler_eff_definition; expand_def;
-    try congruence.
-  find_injection.
-  find_apply_lem_hyp tick_handler_definition; expand_def;
-    try congruence.
-  destruct (start_query _ _ _) as [[[?st' ?ms] ?nts] ?cts] eqn:?H.
-  find_copy_eapply_lem_hyp succ_list_preserved_by_Tick; eauto.
-  repeat find_rewrite.
-  find_eapply_lem_hyp start_query_definition; expand_def.
-  - find_copy_apply_lem_hyp make_request_Stabilize_needs_succ_list; break_exists.
-    repeat find_rewrite.
-    find_injection.
-    eauto using effective_Tick_sends_request.
-  - find_eapply_lem_hyp make_request_Stabilize_None.
-    repeat find_rewrite.
-    congruence.
-Qed.
-
-Lemma get_open_stabilize_request_to_first_succ_from_req_to :
-  forall gst h st dst rest,
-    open_stabilize_request_to gst h (addr_of dst) ->
-    sigma gst h = Some st ->
-    succ_list st = dst :: rest ->
-    open_stabilize_request_to_first_succ gst h.
-Proof.
-  unfold open_stabilize_request_to_first_succ.
-  intros.
-  now repeat (find_injection || find_rewrite).
-Qed.
-
-Lemma effective_Tick_occurred_sent_request :
-  forall h ex,
-    lb_execution ex ->
-    now (occurred (Timeout h Tick StartStabilize)) ex ->
-    next (now (fun o => open_stabilize_request_to_first_succ (occ_gst o) h)) ex.
-Proof.
-  intros.
-  do 2 destruct ex.
-  simpl in *.
-  inv_lb_execution.
-  unfold occurred in *.
-  repeat find_reverse_rewrite.
-  find_copy_apply_lem_hyp timeout_implies_state_exists_after; break_exists_name st'.
-  find_copy_apply_lem_hyp timeout_implies_state_exists; break_exists_name st.
-  destruct (succ_list st') eqn:?H.
-  - congruence.
-  - eapply get_open_stabilize_request_to_first_succ_from_req_to; eauto.
-    eapply effective_Tick_sends_request'; eauto.
-Qed.
-
-Lemma leading_failed_succs_st :
-  forall h gst st,
-    sigma gst h = Some st ->
-    leading_failed_succs h gst = succ_list_leading_failed_nodes (failed_nodes gst) (succ_list st).
-Proof.
-  unfold leading_failed_succs.
-  intros.
-  break_match; congruence.
-Qed.
-
-Lemma stabilize_Request_timeout_removes_succ :
-  forall ex h st s rest dst p,
-    lb_execution ex ->
-    sigma ex.(hd).(occ_gst) h = Some st ->
-    succ_list st = s :: rest ->
-    open_stabilize_request_to ex.(hd).(occ_gst) h dst ->
-    now (occurred (Timeout h (Request dst p) DetectFailure)) ex ->
-    next
-      (now
-         (fun occ =>
-            exists st, sigma occ.(occ_gst) h = Some st /\
-                  succ_list st = rest))
-      ex.
-Proof.
-  intros.
-  unfold open_stabilize_request, open_stabilize_request_to in *; break_exists; break_and.
-  do 2 destruct ex.
-  match goal with
-  | [ H : lb_execution _ |- _ ] =>
-    inv H; simpl in *
-  end.
-  unfold occurred in *.
-  repeat find_reverse_rewrite.
-  invc_labeled_step; simpl in *.
-
-  (* This should be a lemma about timeout_handler_l. *)
-  assert (h0 = h).
-  {
-    find_apply_lem_hyp timeout_handler_l_definition; expand_def.
-    now find_injection.
-  }
-  subst_max.
-  repeat find_rewrite; simpl.
-  rewrite update_same.
-  eexists; split; eauto.
-  find_injection.
-
-  find_apply_lem_hyp timeout_handler_l_definition; expand_def.
-  repeat find_reverse_rewrite.
-  find_injection.
-
-  clear H11.
-  inv_prop open_request_to; expand_def.
-  inv_prop request_msg_for_query.
-  simpl in *.
-
-  find_apply_lem_hyp request_timeout_handler_definition; expand_def; try congruence.
-  find_eapply_lem_hyp handle_query_timeout_definition; expand_def; try congruence.
-  repeat find_rewrite; repeat find_injection.
-  (* Should use a definition lemma about start_query here. *)
-  unfold start_query, update_query in *.
-  simpl in *.
-  repeat break_match;
-    simpl in *;
-    tuple_inversion;
-    reflexivity.
-Qed.
-
-Lemma removing_head_decreases_failed_node_count :
-  forall gst l gst' s rest,
-    labeled_step_dynamic gst l gst' ->
-    In (addr_of s) (failed_nodes gst) ->
-    succ_list_leading_failed_nodes (failed_nodes gst') rest <
-    succ_list_leading_failed_nodes (failed_nodes gst) (s :: rest).
-Proof.
-  intros.
-  erewrite <- failed_nodes_eq; eauto.
-  simpl.
-  break_if;
-    [|exfalso];
-    auto with arith.
-Qed.
-
-Definition has_dead_first_succ (gst : global_state) (h : addr) (s : pointer) :=
-  exists st,
-    sigma gst h = Some st /\
-    exists rest,
-      succ_list st = s :: rest /\
-      In (addr_of s) (failed_nodes gst).
-
-Lemma has_dead_first_succ_intro :
-  forall gst h s st rest,
-    sigma gst h = Some st ->
-    succ_list st = s :: rest ->
-    In (addr_of s) (failed_nodes gst) ->
-    has_dead_first_succ gst h s.
-Proof.
-  firstorder eauto.
-Qed.
-
-(* TODO(ryan) move to structtact *)
-Lemma hd_error_tl_exists :
-  forall A (l : list A) x,
-    hd_error l = Some x ->
-    exists tl,
-      l = x :: tl.
-Proof.
-  intros.
-  destruct l; simpl in *.
-  - congruence.
-  - eexists; solve_by_inversion.
-Qed.
-
-Lemma stabilize_timeout_means_successor_dead :
-  forall ex h dst,
-    lb_execution ex ->
-    reachable_st (occ_gst (hd ex)) ->
-    now (occurred (Timeout h (Request dst GetPredAndSuccs) DetectFailure)) ex ->
-    exists s,
-      addr_of s = dst /\
-      has_dead_first_succ ex.(hd).(occ_gst) h s.
-Proof.
-  intros.
-  destruct ex as [o [o' ex]].
-  simpl in *.
-  unfold occurred in *.
-  inv_prop lb_execution.
-  repeat find_reverse_rewrite.
-  inv_labeled_step; clean_up_labeled_step_cases.
-  find_apply_lem_hyp timeout_handler_l_definition; expand_def;
-    try congruence.
-  find_apply_lem_hyp timeout_handler_eff_definition; expand_def;
-    try congruence.
-  repeat find_rewrite; find_injection.
-  inv_prop timeout_constraint.
-  find_eapply_lem_hyp stabilize_only_with_first_succ; eauto; break_exists_exists.
-  firstorder.
-  eexists; firstorder eauto.
-  find_apply_lem_hyp hd_error_tl_exists; break_exists_exists; firstorder.
-  now find_rewrite.
-Qed.
-
-Lemma open_request_until_timeout :
-  forall ex h dst,
-    lb_execution ex ->
-    reachable_st (occ_gst (hd ex)) ->
-
-    open_stabilize_request_to ex.(hd).(occ_gst) h dst ->
-    weak_until (now (fun occ => open_stabilize_request_to (occ_gst occ) h dst) /\_
-                ~_ now (occurred (Timeout h (Request dst GetPredAndSuccs) DetectFailure)))
-               (now (fun occ => open_stabilize_request_to (occ_gst occ) h dst) /\_
-                now (occurred (Timeout h (Request dst GetPredAndSuccs) DetectFailure)))
-               ex.
-Proof.
-Admitted.
-
-Lemma stabilize_Request_timeout_decreases_error :
-  forall ex h dst,
-    lb_execution ex ->
-    reachable_st (occ_gst (hd ex)) ->
-
-    open_stabilize_request_to ex.(hd).(occ_gst) h dst ->
-    now (occurred (Timeout h (Request dst GetPredAndSuccs) DetectFailure)) ex ->
-    consecutive (measure_decreasing (leading_failed_succs h)) ex.
-Proof.
-  intros.
-  find_copy_eapply_lem_hyp stabilize_timeout_means_successor_dead; eauto.
-  break_exists_name s; break_and.
-  inv_prop has_dead_first_succ; expand_def.
-  destruct ex as [o [o' ex]].
-  find_copy_eapply_lem_hyp stabilize_Request_timeout_removes_succ; eauto.
-  simpl in *; break_exists; break_and.
-  unfold measure_decreasing.
-  erewrite !leading_failed_succs_st; eauto.
-  repeat find_rewrite.
-  inv_prop lb_execution.
-  eapply removing_head_decreases_failed_node_count; eauto.
-Qed.
-
-Lemma start_stabilize_with_first_successor_eventually :
-  forall ex h,
-    lb_execution ex ->
-    reachable_st (occ_gst (infseq.hd ex)) ->
-    strong_local_fairness ex ->
-    always (~_ (now circular_wait)) ex ->
-
-    live_node (occ_gst (hd ex)) h ->
-
-    eventually (now (fun o => open_stabilize_request_to_first_succ o.(occ_gst) h)) ex.
-Proof.
-  intros.
-  find_copy_apply_lem_hyp loaded_Tick_inf_often; auto.
-  inv_prop inf_occurred.
-  eapply eventually_next.
-  lift_eventually (effective_Tick_occurred_sent_request h).
-  invar_eauto.
-Qed.
-
+(* this isn't used anywhere but might be useful in the future *)
 Lemma request_always_effective :
   forall s eff h dst dstp q msg msg' st,
     lb_execution s ->
@@ -910,244 +149,6 @@ Proof.
   congruence.
 Qed.
 
-Lemma zero_error_implies_phase_one :
-  forall ex,
-    lb_execution ex ->
-    reachable_st (occ_gst (hd ex)) ->
-    now (measure_zero phase_one_error) ex ->
-    now phase_one ex.
-Proof.
-  intros.
-  destruct ex.
-  simpl in *.
-  eapply zero_leading_failed_nodes_implies_all_first_succs_best; eauto.
-  eapply nodes_have_nonempty_succ_lists; eauto.
-Qed.
-
-Theorem continuously_zero_total_leading_failed_nodes_implies_phase_one :
-  forall ex,
-    lb_execution ex ->
-    reachable_st (occ_gst (infseq.hd ex)) ->
-    infseq.continuously (now (measure_zero phase_one_error)) ex ->
-    continuously (now phase_one) ex.
-Proof.
-  intros.
-  pose proof zero_error_implies_phase_one.
-  unfold continuously in *.
-  prep_always_monotonic.
-  eapply eventually_monotonic_simple.
-  eapply always_monotonic; eauto.
-  eapply continuously_and_tl; eauto.
-  apply E0.
-  eapply reachable_st_always; eauto.
-Qed.
-
-Theorem phase_one_error_continuously_nonincreasing :
-  forall ex,
-    lb_execution ex ->
-    reachable_st (occ_gst (infseq.hd ex)) ->
-    strong_local_fairness ex ->
-    always (~_ (now circular_wait)) ex ->
-    continuously (local_measures_nonincreasing leading_failed_succs) ex.
-Proof.
-Admitted.
-
-Lemma succ_list_leading_failed_nodes_nonzero_means_dead_succ :
-  forall failed succs,
-    succ_list_leading_failed_nodes failed succs > 0 ->
-    exists p rest,
-      succs = p :: rest /\
-      In (addr_of p) failed.
-Proof.
-  unfold succ_list_leading_failed_nodes.
-  destruct succs; intros.
-  - omega.
-  - break_if.
-    + eexists; eauto.
-    + omega.
-Qed.
-
-Lemma leading_failed_succs_nonzero_means_dead_succ :
-  forall h gst,
-    leading_failed_succs h gst > 0 ->
-    exists st,
-      sigma gst h = Some st /\
-      exists p rest,
-        succ_list st = p :: rest /\
-        In (addr_of p) (failed_nodes gst).
-Proof.
-  unfold leading_failed_succs.
-  intros.
-  break_match; [|omega].
-  eexists; split; eauto.
-  now apply succ_list_leading_failed_nodes_nonzero_means_dead_succ.
-Qed.
-
-Lemma phase_one_error_nonzero_means_dead_succ :
-  forall gst,
-    phase_one_error gst > 0 ->
-    exists h,
-      In h (nodes gst) /\
-      ~ In h (failed_nodes gst) /\
-      exists st,
-        sigma gst h = Some st /\
-        exists p rest,
-          succ_list st = p :: rest /\
-          In (addr_of p) (failed_nodes gst).
-Proof.
-  intros.
-  find_apply_lem_hyp sum_nonzero_implies_addend_nonzero.
-  break_exists; break_and.
-  find_eapply_lem_hyp Coqlib.list_in_map_inv.
-  break_exists_exists.
-  firstorder using in_active_in_nodes, in_active_not_failed.
-  apply leading_failed_succs_nonzero_means_dead_succ; omega.
-Qed.
-
-Lemma has_dead_first_succ_implies_error_nonzero :
-  forall gst h s,
-    has_dead_first_succ gst h s ->
-    leading_failed_succs h gst > 0.
-Proof.
-  unfold has_dead_first_succ.
-  intros.
-  expand_def.
-  unfold leading_failed_succs, succ_list_leading_failed_nodes.
-  repeat find_rewrite.
-  break_if; [|exfalso];
-    auto with arith.
-Qed.
-
-(* TODO(ryan) move to infseq *)
-Lemma weak_until_latch_eventually :
-  forall T (P Q : infseq T -> Prop) ex,
-    weak_until (P /\_ ~_ Q) (P /\_ Q) ex ->
-    eventually Q ex ->
-    eventually (P /\_ Q) ex.
-Proof.
-  induction 2.
-  - inv_prop weak_until.
-    + now apply E0.
-    + exfalso; firstorder.
-  - inv_prop weak_until.
-    + now apply E0.
-    + eauto using E_next.
-Qed.
-
-Lemma open_stabilize_request_eventually_decreases_error :
-  forall ex h,
-    lb_execution ex ->
-    reachable_st (occ_gst (infseq.hd ex)) ->
-    strong_local_fairness ex ->
-    always (~_ (now circular_wait)) ex ->
-
-    live_node (occ_gst (hd ex)) h ->
-
-    leading_failed_succs h (occ_gst (hd ex)) > 0 ->
-    open_stabilize_request_to_first_succ (occ_gst (hd ex)) h ->
-    eventually (consecutive (measure_decreasing (leading_failed_succs h))) ex.
-Proof.
-  intros.
-  find_copy_apply_lem_hyp leading_failed_succs_nonzero_means_dead_succ; expand_def.
-  assert (exists s, has_dead_first_succ (occ_gst (hd ex)) h s)
-    by (repeat eexists; eauto); break_exists_name s.
-  unfold open_stabilize_request_to_first_succ in *.
-  find_copy_apply_hyp_hyp.
-  find_copy_eapply_lem_hyp open_request_until_timeout; eauto.
-  find_copy_apply_lem_hyp request_eventually_fires;
-    eauto using strong_local_fairness_weak.
-  find_copy_apply_lem_hyp eventually_weak_until_cumul; eauto.
-  find_copy_apply_lem_hyp reachable_st_always; auto.
-  eapply eventually_monotonic; [| | eauto | eauto]; intros.
-  - invar_eauto.
-  - invc_prop always.
-    unfold and_tl in *; break_and.
-    invcs_prop weak_until; break_and;
-      destruct s0;
-      eapply stabilize_Request_timeout_decreases_error; eauto.
-  - eapply weak_until_latch_eventually; eauto.
-Qed.
-
-Lemma nonzero_error_eventually_drops :
-  forall ex h,
-    lb_execution ex ->
-    reachable_st (occ_gst (infseq.hd ex)) ->
-    strong_local_fairness ex ->
-    always (~_ (now circular_wait)) ex ->
-
-    live_node (occ_gst (hd ex)) h ->
-    leading_failed_succs h (occ_gst (hd ex)) > 0 ->
-
-    eventually (consecutive (measure_decreasing (leading_failed_succs h))) ex.
-Proof.
-  intros.
-  find_copy_eapply_lem_hyp start_stabilize_with_first_successor_eventually; eauto.
-  induction 0.
-  - destruct s.
-    eapply open_stabilize_request_eventually_decreases_error; eauto.
-  - destruct s as [o' s].
-    destruct (leading_failed_succs h (occ_gst o')) eqn:?H.
-    + apply E0.
-      simpl in *.
-      unfold measure_decreasing.
-      omega.
-    + apply E_next.
-      apply IHeventually; invar_eauto.
-      simpl; omega.
-Qed.
-
-Lemma nonempty_succ_list_implies_joined :
-  forall gst h st s rest,
-    reachable_st gst ->
-    sigma gst h = Some st ->
-    succ_list st = s :: rest ->
-    joined st = true.
-Proof.
-  intros.
-  destruct (joined st) eqn:?H;
-    [|find_apply_lem_hyp nodes_not_joined_have_no_successors; auto];
-    congruence.
-Qed.
-
-Theorem phase_one_nonzero_error_causes_measure_drop :
-  forall ex,
-    lb_execution ex ->
-    reachable_st (occ_gst (infseq.hd ex)) ->
-    strong_local_fairness ex ->
-    always (~_ (now circular_wait)) ex ->
-    always (nonzero_error_causes_measure_drop leading_failed_succs) ex.
-Proof.
-  cofix c.
-  intros.
-  destruct ex.
-  constructor.
-  - intro.
-    find_copy_apply_lem_hyp phase_one_error_nonzero_means_dead_succ.
-    break_exists_exists; expand_def.
-    split; auto using in_nodes_not_failed_in_active.
-    eapply nonzero_error_eventually_drops; eauto.
-    + find_eapply_lem_hyp nonempty_succ_list_implies_joined;
-        eauto using live_node_characterization.
-    + eauto using has_dead_first_succ_intro, has_dead_first_succ_implies_error_nonzero.
-  - simpl.
-    apply c; invar_eauto.
-Qed.
-
-Theorem phase_one_continuously :
-  forall ex,
-    lb_execution ex ->
-    reachable_st (occ_gst (infseq.hd ex)) ->
-    strong_local_fairness ex ->
-    always (~_ (now circular_wait)) ex ->
-    continuously (now phase_one) ex.
-Proof.
-  intros.
-  eapply continuously_zero_total_leading_failed_nodes_implies_phase_one; eauto.
-  eapply local_measure_causes_measure_zero_continuosly; eauto.
-  - eapply phase_one_error_continuously_nonincreasing; eauto.
-  - eauto using always_continuously, phase_one_nonzero_error_causes_measure_drop.
-Qed.
-
 (** In phase two we want to talk about the existence and number of better
     predecessors and better first successors to a node. We do this with the
     following functions.
@@ -1162,7 +163,7 @@ Qed.
 Definition counting_opt_error (gst : global_state) (p : option pointer) (better_bool : pointer -> pointer -> bool) : nat :=
   match p with
   | Some p0 =>
-    if live_dec gst p0
+    if live_node_dec gst (addr_of p0)
     then length (filter (better_bool p0) (live_ptrs gst))
     else length (live_ptrs gst) + 1
   | None => length (live_ptrs gst) + 1
@@ -1174,7 +175,8 @@ Lemma counting_opt_error_zero_implies_correct :
     exists p0,
       p = Some p0 /\
       forall p',
-        live gst p' ->
+        live_node gst (addr_of p') ->
+        wf_ptr p' ->
         better_bool p0 p' = false.
 Proof.
   unfold counting_opt_error.
@@ -1184,7 +186,10 @@ Admitted.
 
 (** Predecessor phase two definitions *)
 Definition better_pred (gst : global_state) (h p p' : pointer) : Prop :=
-  live gst p' /\ ptr_between p p' h.
+  wf_ptr p /\
+  wf_ptr p' /\
+  live_node gst (addr_of p') /\
+  ptr_between p p' h.
 
 Definition better_pred_bool (h p p' : pointer) : bool :=
   ptr_between_bool p p' h.
@@ -1200,7 +205,10 @@ Definition pred_error (gst : global_state) (h : pointer) (p : option pointer) : 
 
 (** First successor phase two definitions *)
 Definition better_succ (gst : global_state) (h s s' : pointer) : Prop :=
-  live gst s' /\ ptr_between h s' s.
+  wf_ptr s /\
+  wf_ptr s' /\
+  live_node gst (addr_of s') /\
+  ptr_between h s' s.
 
 Definition better_succ_bool (h s s' : pointer) : bool :=
   ptr_between_bool h s' s.
@@ -1232,13 +240,15 @@ Definition phase_two_error : global_state -> nat :=
 
 Definition preds_and_first_succs_correct (gst : global_state) : Prop :=
   forall h st,
-    live gst h ->
+    live_node gst (addr_of h) ->
+    wf_ptr h ->
     sigma gst (addr_of h) = Some st ->
     pred_and_first_succ_correct gst h st.
 
 Lemma phase_two_zero_error_locally_correct :
   forall gst h st,
-    live gst h ->
+    live_node gst (addr_of h) ->
+    wf_ptr h ->
     sigma gst (addr_of h) = Some st ->
     pred_and_first_succ_error (addr_of h) gst = 0 ->
     pred_and_first_succ_correct gst h st.
@@ -1259,11 +269,11 @@ Qed.
 
 Lemma live_In_live_ptrs :
   forall gst h,
-    live gst h ->
+    live_node gst (addr_of h) ->
     wf_ptr h ->
     In h (live_ptrs gst).
 Proof.
-  unfold live_ptrs, live.
+  unfold live_ptrs, live_node.
   intros.
   rewrite (wf_ptr_eq h); auto.
   apply in_map.
@@ -1272,8 +282,8 @@ Qed.
 
 Lemma live_In_live_ptrs_with_states :
   forall gst h st,
+    live_node gst (addr_of h) ->
     wf_ptr h ->
-    live gst h ->
     sigma gst (addr_of h) = Some st ->
     In (h, st) (live_ptrs_with_states gst).
 Proof.
@@ -1369,13 +379,14 @@ Definition correct_succs (gst : global_state) (h : pointer) (st : data) : Prop :
     wf_ptr h ->
     succ_list st = xs ++ s :: ys ->
     ptr_between h s' s ->
-    live gst s' ->
+    live_node gst (addr_of s') ->
     In s' xs.
 
 Definition all_succs_correct (gst : global_state) : Prop :=
   forall h st,
     sigma gst (addr_of h) = Some st ->
-    live gst h ->
+    live_node gst (addr_of h) ->
+    wf_ptr h ->
     correct_succs gst h st /\
     length (succ_list st) = Chord.SUCC_LIST_LEN.
 
@@ -1398,7 +409,8 @@ Admitted.
 
 Definition ideal (gst : global_state) : Prop :=
   forall h st,
-    live gst h ->
+    live_node gst (addr_of h) ->
+    wf_ptr h ->
     sigma gst (addr_of h) = Some st ->
     correct_succs gst h st /\
     length (succ_list st) = Chord.SUCC_LIST_LEN /\
